no_redex => has_redex

FokkerChallenge/Basic.lean
@@ -20,48 +20,6 @@ induction M with (unfold openRec fokker_size; grind)
 def r_preserves (f: Term String -> Bool) (R : Term String → Term String → Prop) : Prop :=
   ∀ M N, R M N → f M → f N
 
-def no_redex: Term String → Bool
-  | Term.bvar _ => true
-  | Term.fvar _ => true
-  | Term.abs t => no_redex t
-  | Term.app (Term.abs _) _ => false
-  | Term.app t1 t2 => no_redex t1 && no_redex t2
-
-/-
-theorem no_redex_false_equiv_full_beta {M}: no_redex M = false <-> ∃ N, FullBeta M N := by
-induction M with
-| bvar _ => unfold no_redex
-            simp
-            intros _ h
-            cases h
-            rename_i h
-            cases h
-| fvar _ => unfold no_redex
-            simp
-            intros _ h
-            cases h
-            rename_i h
-            cases h
-| abs M ih => unfold no_redex
-              rw [ih]
-              constructor <;> intros h <;> obtain ⟨N, h⟩ := h
-              . exists N.abs
-                apply Xi.abs M.fv
-                intros x _
-                unfold open'
-                rw [<- Cslib.LambdaCalculus.LocallyNameless.Untyped.Term.open_lc]
-                rw [<- Cslib.LambdaCalculus.LocallyNameless.Untyped.Term.open_lc]
-                assumption
-                . apply Cslib.LambdaCalculus.LocallyNameless.Untyped.Term.FullBeta.step_lc_r h
-                . apply Cslib.LambdaCalculus.LocallyNameless.Untyped.Term.FullBeta.step_lc_l h
-              . cases h with
-                | base h => cases h
-                | abs xs h => rename_i N
-                              exists N
-                              -- impossible to prove
-                              sorry
-| app _ _ _ _ => sorry
--/
 
 /-
   K = λx y. x
