FokkerChallenge/EnhancedCslib/NormalForm.lean
@@ -1,0 +1,26 @@
+import Cslib.Languages.LambdaCalculus.LocallyNameless.Untyped.Basic
+import Cslib.Languages.LambdaCalculus.LocallyNameless.Untyped.FullBeta
+import Cslib.Languages.LambdaCalculus.LocallyNameless.Untyped.Congruence
+import Cslib.Languages.LambdaCalculus.LocallyNameless.Untyped.FullBetaEtaConfluence
+import FokkerChallenge.EnhancedCslib.Basic
+import Mathlib.Data.Finset.Lattice.Basic
+
+namespace Cslib
+
+namespace LambdaCalculus.LocallyNameless.Untyped.Term
+
+def has_redex: Term String → Bool
+  | Term.bvar _ => false
+  | Term.fvar _ => false
+  | Term.abs t => has_redex t
+  | Term.app (Term.abs _) _ => true
+  | Term.app t1 t2 => has_redex t1 || has_redex t2
+
+theorem has_redex_equiv_full_beta {M}: has_redex M /\ M.LC <-> ∃ N, FullBeta M N := by
+sorry
+
+theorem no_redex_refl {M N}: has_redex M = false -> Relation.ReflTransGen FullBeta M N -> M = N := by
+sorry
+
+theorem reflTransGen_iff_eqvGen_of_normal {M N: Term String} (hn: N.has_redex = false) : Relation.ReflTransGen FullBetaEta M N.abs ↔ Relation.EqvGen FullBetaEta M N.abs := by
+sorry
